Cslib/Computability/Machines/MultiTapeTuring/IsZeroRoutine.lean
@@ -1,0 +1,32 @@
+/-
+Copyright (c) 2026 Christian Reitwiessner. All rights reserved.
+Released under Apache 2.0 license as described in the file LICENSE.
+Authors: Christian Reitwiessner
+-/
+
+module
+
+public import Cslib.Computability.Machines.MultiTapeTuring.Basic
+public import Cslib.Computability.Machines.MultiTapeTuring.ListEncoding
+public import Cslib.Computability.Machines.MultiTapeTuring.PushRoutine
+public import Cslib.Computability.Machines.MultiTapeTuring.PopRoutine
+public import Cslib.Computability.Machines.MultiTapeTuring.SequentialCombinator
+public import Cslib.Computability.Machines.MultiTapeTuring.IteCombinator
+
+namespace Turing
+
+variable {k : ℕ}
+
+namespace Routines
+
+public def isZero (i : Fin k) := ite i (pop i <;> push i []) (pop i <;> push i [OneTwo.one])
+
+@[simp, grind =]
+public theorem isZero_eval_list {i : Fin k} {tapes : Fin k → List (List OneTwo)} :
+  (isZero i).eval_list tapes = .some (Function.update tapes i (
+    (if (tapes i).headD [] = [] then [OneTwo.one] else []) :: (tapes i).tail)) := by
+  simp [isZero]
+  grind
+
+end Routines
+end Turing
